Core/Examples/Boolean.lean
@@ -106,12 +106,12 @@ def t1 : Term := ((openm! "eq" #( gt#"Bool" ) #() (Vec.to (#( iBool )))) • Tru
 #guard t1.infer_type EqBoolCtx [] [] == some (gt#"Bool")
 -- def t2 : Term := (g#"eq" •[ gt#"Bool" ]  • (g#"EqBool" •[  gt#"Bool" ] • refl! gt#"Bool") • g#"True") • g#"True"
 
-#eval t1.eval_loop EqBoolCtx
+#guard t1.eval_loop EqBoolCtx == some (FalseCtor)
 
-#eval do
-  let ctors <- Term.is_data .opn #(iBool)
-  return (ctors, EqBoolCtx[0]?)
-  -- get_instance "eq" ctors EqBoolCtx
+-- #eval do
+--   let ctors <- Term.is_data .opn #(iBool)
+--   return (ctors, EqBoolCtx[0]?)
+--   -- get_instance "eq" ctors EqBoolCtx
 
 
 
@@ -132,7 +132,7 @@ def t3 : Term := ((openm! "eq" #( gt#"Bool") #() (Vec.to (#(iBool)))) • TrueCt
 #guard t3.eval_loop EqBoolCtx == FalseCtor
 
 
-#guard EqBoolCtx.check_open_exhaustive == some ()
+#guard EqBoolCtx.check_open_exhaustive.isSome
 
 
 
